theories/lang/primitive_laws.v
@@ -11,7 +11,7 @@ From self.lang Require Import notation.
 
 Class nvmG Σ := NvmG {
   nvmG_invG : invG Σ;
-  nvmG_gen_heapG :> gen_heapG loc (@history val) Σ;
+  nvmG_gen_heapG :> gen_heapG loc history Σ;
   view_inG :> inG Σ (authR viewUR);
   (* heapG_inv_heapG :> inv_heapG loc (option val) Σ; *)
   nvmG_proph_mapG :> proph_mapG proph_id (val * val) Σ;
@@ -19,7 +19,7 @@ Class nvmG Σ := NvmG {
   persist_view_name : gname;
 }.
 
-Definition max_msg (h : @history val) : time :=
+Definition max_msg (h : history) : time :=
   max_list (elements (dom (gset time) h)).
 
 Lemma max_list_elem_of ns : ns ≠ [] → max_list ns ∈ ns.
@@ -53,7 +53,13 @@ Lemma lookup_max_msg (hist : history) :
   is_Some (hist !! 0) → is_Some (hist !! max_msg hist).
 Proof. apply lookup_max_msg_helper. Qed.
 
-Definition lub_view (heap : (@store val)) : view := max_msg <$> heap.
+Definition lub_view (heap : store) : gmap loc max_nat := MaxNat <$> (max_msg <$> heap).
+
+Definition hist_inv heap hist `{!nvmG Σ} : iProp Σ :=
+  ( (* Every history has an initial message. *)
+    ⌜is_Some (hist !! 0)⌝ ∗
+    (* Every view in every message is included in the lub view. *)
+    ([∗ map] t ↦ msg ∈ hist, ⌜msg.(msg_store_view) ⊑ lub_view heap⌝))%I.
 
 Global Instance nvmG_irisG `{!nvmG Σ} : irisG nvm_lang Σ := {
   iris_invG := nvmG_invG;
@@ -61,12 +67,12 @@ Global Instance nvmG_irisG `{!nvmG Σ} : irisG nvm_lang Σ := {
     (* The interpetation of the heap. This is standard, except the heap store
     historie and not plain values. *)
     gen_heap_interp (fst σ) ∗
-    own store_view_name (● (view_to_ra (lub_view (fst σ)))) ∗
-    ([∗ map] ℓ ↦ hist ∈ (fst σ),
+    own store_view_name (● (lub_view (fst σ))) ∗
+    ([∗ map] ℓ ↦ hist ∈ (fst σ), hist_inv (fst σ) hist) ∗
       (* Every history has an initial message. *)
-      ⌜is_Some (hist !! 0)⌝ ∗
+      (* ⌜is_Some (hist !! 0)⌝ ∗ *)
       (* Every view in every message is included in the lub view. *)
-      ([∗ map] t ↦ msg ∈ hist, ⌜msg.(msg_store_view) ⊑ lub_view (fst σ)⌝)) ∗
+      (* ([∗ map] t ↦ msg ∈ hist, ⌜msg.(msg_store_view) ⊑ lub_view (fst σ)⌝)) ∗ *)
     (*
     (* There exists some "all-knowing" view [W]. *)
     (∃ W, (* We know what [W] is. *)
@@ -75,7 +81,7 @@ Global Instance nvmG_irisG `{!nvmG Σ} : irisG nvm_lang Σ := {
                                        ([∗ map] t ↦ msg ∈ hist, ⌜msg.(msg_store_view) ⊑ W⌝)) ∗
           ⌜∀ ℓ t hist, (W !!0 ℓ ) = t ∧ ((fst σ) !! ℓ) = Some hist ∧ is_Some (hist !! t)⌝) ∗
     *)
-    own persist_view_name (● (view_to_ra (snd σ)))
+    own persist_view_name (● (snd σ))
     (* proph_map_interp κs σ.(used_proph_id) *)
   )%I;
   fork_post _ := True%I;
@@ -88,28 +94,35 @@ Notation "l ↦h□ v" := (mapsto (L:=loc) (V:=val) l DfracDiscarded (Some v%V))
   (at level 20, format "l  ↦h□  v") : bi_scope.
 Notation "l ↦h{# q } v" := (mapsto (L:=loc) (V:=val) l (DfracOwn q) (Some v%V))
   (at level 20, format "l  ↦h{# q }  v") : bi_scope. *)
-Notation "l ↦h v" := (mapsto (L:=loc) (V:=(@history val)) l (DfracOwn 1) (v%V))
+Notation "l ↦h v" := (mapsto (L:=loc) (V:=history) l (DfracOwn 1) (v%V))
   (at level 20, format "l  ↦h  v") : bi_scope.
 
 Section lifting.
 
   Context `{!nvmG Σ}.
 
-  Definition valid (V : view) : iProp Σ := own store_view_name (◯ (view_to_ra V)).
+  Implicit Types Q : iProp Σ.
+  Implicit Types Φ Ψ : val → iProp Σ.
+  Implicit Types efs : list expr.
+  (* Implicit Types σ : state. *)
+  Implicit Types v : val.
+  Implicit Types ℓ : loc.
+
+  Definition valid (V : view) : iProp Σ := own store_view_name (◯ V).
 
   Global Instance valid_persistent V : Persistent (valid V).
   Proof. apply _. Qed.
 
-  Definition persisted (V : view) : iProp Σ := own persist_view_name (◯ (view_to_ra V)).
+  Definition persisted (V : view) : iProp Σ := own persist_view_name (◯ V).
 
   Global Instance persisted_persistent V : Persistent (persisted V).
   Proof. apply _. Qed.
 
-  Lemma auth_frag_leq V W γ : ⊢ own γ (◯ (view_to_ra V)) -∗ own γ (● view_to_ra W) -∗ ⌜V ⊑ W⌝.
+  Lemma auth_frag_leq V W γ : ⊢ own γ (◯ V) -∗ own γ (● W) -∗ ⌜V ⊑ W⌝.
   Proof.
     iIntros "H1 H2".
     rewrite /valid.
-    iDestruct (own_valid_2 with "H2 H1") as %[Hincl%view_to_ra_incl _]%auth_both_valid_discrete.
+    iDestruct (own_valid_2 with "H2 H1") as %[Hincl _]%auth_both_valid_discrete.
     done.
   Qed.
 
@@ -119,16 +132,37 @@ Section lifting.
     heap !! ℓ = Some hist → is_Some (hist !! 0) → is_Some (hist !! ((lub_view heap) !!0 ℓ)).
   Proof.
     intros Ha Hb.
-    rewrite /lub_view. rewrite lookup_fmap. rewrite Ha.
+    rewrite /lub_view. rewrite !lookup_fmap. rewrite Ha.
     simpl. apply lookup_max_msg_helper. done.
   Qed.
 
-  Implicit Types Q : iProp Σ.
-  Implicit Types Φ Ψ : val → iProp Σ.
-  Implicit Types efs : list expr.
-  (* Implicit Types σ : state. *)
-  Implicit Types v : val.
-  Implicit Types ℓ : loc.
+  Lemma store_view_alloc_big (σ σ' : (gmap loc history)) :
+    σ' ##ₘ σ →
+    own store_view_name (● (lub_view (σ))) ==∗
+    own store_view_name (● (lub_view (σ' ∪ σ))).
+  Proof.
+  Admitted.
+
+  Lemma hist_inv_alloc ℓ P v0 n heap :
+    heap_array ℓ P (replicate (Z.to_nat n) v0) ##ₘ heap →
+    ([∗ map] hist ∈ heap, hist_inv heap hist) -∗
+    ([∗ map] hist ∈ (heap_array ℓ P (replicate (Z.to_nat n) v0) ∪ heap),
+      hist_inv (heap_array ℓ P (replicate (Z.to_nat n) v0) ∪ heap) hist).
+  Proof.
+    iIntros (disj) "H".
+    rewrite big_sepM_union; last apply disj.
+    iSplitR "H".
+    - iApply big_sepM_intuitionistically_forall.
+      iIntros (ℓ' hist) "!> %".
+      admit.
+    - iApply (big_sepM_impl with "H").
+    (* - iApply (big_sepM_wand with "H"). *)
+      (* iApply big_sepM_intuitionistically_forall. *)
+      iIntros (ℓ' hist) "!> % [% H]".
+      iSplit; first done.
+      iApply (big_sepM_impl with "H").
+      iIntros (t msg) "!> % %".
+  Admitted.
 
   (* Create a message from a [value] and a [thread_view]. *)
   Definition mk_message (v : val) (T : thread_view) := Msg v T.(tv_store_view) T.(tv_persist_view).
@@ -171,7 +205,7 @@ Section lifting.
     rewrite big_opM_singleton; iDestruct "Hvs" as "[$ Hvs]". by iApply "IH".
   Qed.
 
-  Lemma wp_allocN v T (hist : (@history val)) n s E :
+  Lemma wp_allocN v T (hist : history) n s E :
     (0 < n)%Z →
     {{{ True }}}
       (ThreadState (AllocN #n v) T) @ s; E
@@ -179,7 +213,7 @@ Section lifting.
   Proof.
     iIntros (Hn Φ) "_ HΦ".
     iApply (wp_lift_atomic_head_step_no_fork (_)); first done.
-    iIntros ([??] κ κs k) "[Hσ Hσse] !>"; iSplit.
+    iIntros ([??] κ κs k) "(Hσ & Hauth & Hop & Hpers) !>"; iSplit.
     - (* We must show that [ref v] is can take tome step. *)
        rewrite /head_reducible.
        destruct T.
@@ -189,34 +223,37 @@ Section lifting.
        * apply alloc_fresh. lia.
     - iNext. iIntros (e2 σ2 efs Hstep).
       simpl in *. inv_thread_step. iSplitR=>//.
-      (* We now update the [gen_heap] ghost state to include the allocated location. *)
-      iMod (gen_heap_alloc_big _ (heap_array ℓ _ (replicate (Z.to_nat n) v0)) with "Hσ")
-        as "(Hσ & Hl & Hm)".
+      assert (heap_array ℓ P (replicate (Z.to_nat n) v0) ##ₘ g) as Hdisj.
       { apply heap_array_map_disjoint.
         rewrite replicate_length Z2Nat.id; auto with lia. }
-      iModIntro.
+      iFrame "Hpers".
+      (* We now update the [gen_heap] ghost state to include the allocated location. *)
+      iMod (gen_heap_alloc_big with "Hσ") as "(Hσ & Hl & Hm)"; first apply Hdisj.
       iFrame "Hσ".
-      (* FIXME: This changed after state interpretation changed. *)
-  Abort.
-      (* iFrame "Hσse". iApply "HΦ".
-      iApply heap_array_to_seq_mapsto.
-      iFrame.
-  Qed. *)
+      rewrite /state_init_heap.
+      iMod (store_view_alloc_big with "Hauth") as "$".
+      { apply Hdisj. }
+      iModIntro.
+      iDestruct (hist_inv_alloc with "Hop") as "Hop"; first apply Hdisj.
+      iFrame "Hop".
+      iApply "HΦ". iApply heap_array_to_seq_mapsto. iFrame.
+  Qed.
 
   (* Non-atomic load. *)
-  Lemma wp_load V p B ℓ (hist : (@history val)) s E :
+  Lemma wp_load V p B ℓ (hist : history) s E :
     {{{ ℓ ↦h hist ∗ valid V }}}
       (ThreadState (! #ℓ) (ThreadView V p B)) @ s; E
     {{{ t v, RET (ThreadVal v (ThreadView V p B)); ⌜msg_val <$> (hist !! t) = Some v ∧ (V !!0 ℓ) ≤ t⌝ }}}.
   Proof.
     iIntros (Φ) "[ℓPts Hval] HΦ".
     iApply (wp_lift_atomic_head_step_no_fork (_)); first done.
-    iIntros ([heap ?] κ κs k) "(Hheap & lubauth & #Hincl & persist) /= !>"; iSplit.
+    iIntros ([heap ?] κ κs k) "(Hheap & lubauth & #Hincl & persist) /= !>".
+    (* From the points-to predicate we know that [hist] is in the heap at ℓ. *)
+    iDestruct (gen_heap_valid with "Hheap ℓPts") as %Hlook.
+    iSplit.
     - (* We must show that the load can take some step. To do this we must use
          the points-to predicate and fact that the view is valid. *)
       rewrite /head_reducible.
-      (* From the points-to predicate we know that [hist] is in the heap at ℓ. *)
-      iDestruct (gen_heap_valid with "Hheap ℓPts") as %Hlook.
       (* We need to show that there is _some_ message that the load could read.
       It could certainly read the most recent message. *)
       iAssert (⌜is_Some (hist !! 0)⌝%I) as %HisS.
@@ -230,16 +267,12 @@ Section lifting.
       * econstructor; last by apply view_lt_lt.
         + done.
         + rewrite Hmsgeq. done.
-    - iNext. iIntros (e2 σ2 efs Hstep).
+    - iNext. iIntros (e2 σ2 efs Hstep) "!>".
       simpl in *. inv_thread_step. iSplitR=>//.
-      (* We now update the [gen_heap] ghost state to include the allocated location. *)
-      iMod (gen_heap_alloc_big _ (heap_array ℓ _ (replicate (Z.to_nat n) v0)) with "Hσ")
-        as "(Hσ & Hl & Hm)".
-      { apply heap_array_map_disjoint.
-        rewrite replicate_length Z2Nat.id; auto with lia. }
-      iModIntro.
-      iFrame "Hσ".
-  Abort.
+      (* assert (h = hist) as ->. { rewrite Hlook in H9. congruence. } *)
+      iFrame "Hheap lubauth persist Hincl".
+      by iApply "HΦ".
+  Qed.
 
   Lemma wp_load_acquire V p B ℓ (hist : (@history val)) s E :
     {{{ ℓ ↦h hist ∗ valid V }}}
