theories/algebra/view.v
@@ -1,41 +1,77 @@
 From stdpp Require Import countable numbers gmap.
 From iris.heap_lang Require Export locations.
-From iris.algebra Require Import auth gmap numbers.
+From iris.algebra Require Export gmap numbers.
 
 Notation time := nat.
 
-Notation view := (gmap loc time).
+(* A view is a finite map from locations to natural numbers. A view is a monoid
+  with the empty map as the unit and point-wise max as the operation. To get
+  this monoid structure very easily we use the camera of finite maps and the
+  max_nat camera. We will use this definition in, for instance, the memory model
+  where the full camera structure is not needed. But, this approach simplifies
+  things greatly. *)
+Notation view := (gmap loc max_nat).
+
+Notation viewUR := (gmapUR loc max_natUR).
 
 Implicit Types (V W : view) (ℓ : loc).
 
-Instance join_view : Join view := (union_with (λ (x1 x2 : nat), Some (x1 `max` x2))).
+(* Definition maybe_max mx my :=
+  match mx, my withtime
+  | Some x, Some y => Some (x `max` y)
+  | _, _ => None end). *)
 
-Instance subseteq_view : SqSubsetEq view :=
-  λ v w, ∀ k t, v !! k = Some t → ∃ t', w !! k = Some t' ∧ t ≤ t'.
+Instance join_view : Join view :=
+  λ a b, a ⋅ b.
+  (* (merge (λ (x1 x2 : nat), Some (x1 `max` x2))). *)
 
-Lemma view_lt (V W : view) : V ⊑ W ↔ ∃ V', V ⊔ V' = W.
+(* Instance join_view : Join view := (union_with (λ (x1 x2 : nat), Some (x1 `max` x2))). *)
+
+Instance subseteq_view : SqSubsetEq view := λ v w, v ≼ w.
+  (* λ v w, v ⊔ w = w. *)
+  (* λ v w, ∀ k t, v !! k = Some t → ∃ t', w !! k = Some t' ∧ t ≤ t'. *)
+
+Lemma subseteq_view_incl V W : (V ⊑ W) = (V ≼ W).
+Proof. done. Qed.
+
+Global Instance subseteq_view_assoc : Assoc (=) (join_view).
+Proof. apply _. Qed.
+
+(* Global Instance subseteq_view_transitive' : Transitive (subseteq_view).
 Proof.
-Admitted.
+  intros V1 V2 V3. rewrite /subseteq_view.
+  intros H H'. rewrite -H'. rewrite assoc. rewrite H. done.
+Qed. *)
 
-Infix "!!0" := (λ m i, default 0 (m !! i)) (at level 80).
+(* Lemma view_lt (V W : view) : V ⊑ W ↔ ∃ V', V ⊔ V' = W.
+Proof.
+Admitted. *)
+
+Infix "!!0" := (λ m i, default 0 (max_nat_car <$> (m !! i))) (at level 80).
 
 Lemma view_lt_lt V W ℓ : V ⊑ W → (V !!0 ℓ) ≤ (W !!0 ℓ).
 Proof.
-  intros H.
-  destruct (V !! ℓ) as [t|] eqn:Eq; rewrite Eq; simpl.
-  - apply H in Eq as (t' & -> & ?). done.
-  - lia.
+  rewrite subseteq_view_incl lookup_included.
+  intros le.
+  pose proof (le ℓ) as le.
+  move: le.
+  destruct (V !! ℓ) as [[t]|] eqn:eq, (W !! ℓ) as [[t'']|] eqn:eq'; simpl; try lia.
+  - rewrite eq. rewrite eq'.
+    rewrite Some_included_total.
+    rewrite max_nat_included.
+    done.
+  - rewrite eq. rewrite eq'.
+    rewrite option_included.
+    intros [?|[? [? (_ & ? & _)]]]; done.
 Qed.
 
-(* Resource algebra for views. *)
-Definition viewUR := gmapUR loc max_natUR.
+(* Definition view_to_ra (v : view) : view := (@id view). *)
+  (* MaxNat <$> v. *)
 
-Definition view_to_ra (v : view) : viewUR := MaxNat <$> v.
-
-Global Instance view_core_id (v : viewUR) : CoreId v.
+Global Instance view_core_id (v : view) : CoreId v.
 Proof. apply _. Qed.
 
-Lemma view_to_ra_injective V U : view_to_ra V ≡ view_to_ra U → V = U.
+(* Lemma view_to_ra_injective V U : view_to_ra V ≡ view_to_ra U → V = U.
 Proof.
   intros H.
   apply map_eq.
@@ -44,18 +80,18 @@ Proof.
   rewrite !lookup_fmap in Heq.
   destruct (V !! ℓ), (U !! ℓ); try done.
   by inversion Heq.
-Qed.
+Qed. *)
 
-Lemma view_to_ra_surjective U : ∃ V, view_to_ra V ≡ U.
+(* Lemma view_to_ra_surjective U : ∃ V, view_to_ra V ≡ U.
 Proof.
   exists (max_nat_car <$> U). intros K.
   rewrite /view_to_ra. rewrite !lookup_fmap.
   destruct (U !! K) as [[n]|] eqn:Eq; rewrite Eq; done.
-Qed.
+Qed. *)
 
 (* Check view_to_ra_surjective. *)
 
-Lemma view_to_ra_op V W : view_to_ra V ⋅ view_to_ra W = view_to_ra (V ⊔ W).
+(* Lemma view_to_ra_op V W : view_to_ra V ⋅ view_to_ra W = view_to_ra (V ⊔ W).
 Proof.
   apply leibniz_equiv.
   intros K.
@@ -64,10 +100,10 @@ Proof.
   rewrite !lookup_fmap.
   rewrite lookup_union_with.
   destruct (V !! K), (W !! K); done.
-Qed.
+Qed. *)
 
 (* NOTE: The other direction should hold as well. *)
-Lemma view_to_ra_incl V W : view_to_ra V ≼ view_to_ra W → V ⊑ W.
+(* Lemma view_to_ra_incl V W : view_to_ra V ≼ view_to_ra W → V ⊑ W.
 Proof.
   intros [U Heq%leibniz_equiv].
   (* apply view_to_ra_surjective in U. *) (* Why does this now work? *)
@@ -79,4 +115,4 @@ Proof.
   apply view_to_ra_injective.
   rewrite Heq.
   done.
-Qed.
+Qed. *)
